add get_hdom

state/Monotonic.IFC.Heap.fst
@@ -72,6 +72,14 @@ let not_addr_unused_in_nullptr h = ()
 
 let unused_in #a #rel r h = addr_unused_in (addr_of r) h
 
+module FSet = FStar.FiniteSet.Base
+
+let get_hdom h =
+  FSet.all_finite_set_facts_lemma ();
+  let rec aux (n:nat) : res:(FSet.set pos){forall i. 0 < i && i <= n ==> i `FSet.mem` res} =
+    if n = 0 then FSet.emptyset else FSet.singleton n `FSet.union` (aux (n-1)) in
+  aux ((fst h).next_addr-1)
+
 let sel_tot #a #rel (h, _) r =
   let Some (| _, _, _, x |) = h.memory r.addr in
   x
